Continue compiler.

Compiler.thy
@@ -31,6 +31,44 @@ datatype instr =
 | JMPGE int   (* Compare two topmost stack elements and jump if
                  the second one is greater or equal. *)
 
+(* Program configurations *)
+type_synonym stack = "val list"
+type_synonym config = "int \<times> state \<times> stack"
 
+abbreviation "hd2 xs == hd(tl xs)"
+abbreviation "tl2 xs == tl(tl xs)"
+
+fun iexec :: "instr \<Rightarrow> config \<Rightarrow> config" where
+  "iexec (LOADI n) (i, s, stk)   = (i + 1, s, n # stk)"
+| "iexec (LOAD x) (i, s, stk)    = (i +1, s, s x # stk)"
+| "iexec ADD (i, s, stk)         = (i + 1, s, (hd2 stk + hd stk) # tl2 stk)"
+| "iexec (STORE x) (i, s, stk)   = (i + 1, s(x := hd stk), tl stk)"
+| "iexec (JMP n) (i, s, stk)     = (i + 1 + n, s, stk)"
+| "iexec (JMPLESS n) (i, s, stk) = (if hd2 stk < hd stk then i + 1 + n else i + 1, s, tl2 stk)"
+| "iexec (JMPGE n) (i, s, stk)   = (if hd stk \<le> hd2 stk then i + 1 + n else i + 1, s, tl2 stk)"
+
+definition exec1 :: "instr list \<Rightarrow> config \<Rightarrow> config \<Rightarrow> bool" ("(_/ \<turnstile> (_ \<rightarrow>/ _))" [59,0,59] 60)
+where
+  "P \<turnstile> c \<rightarrow> c' =
+  (\<exists>i s stk. c = (i, s, stk) \<and> c' = iexec (P!!i) (i, s, stk) \<and> 0 \<le> i \<and> i < size P)"
+
+lemma exec1I [intro, code_pred_intro]:
+  "c' = iexec (P!!i) (i, s, stk) \<Longrightarrow> 0 \<le> i \<Longrightarrow> i < size P \<Longrightarrow>
+   P \<turnstile> (i, s, stk) \<rightarrow> c'"
+by (simp add: exec1_def)
+
+abbreviation
+  exec :: "instr list \<Rightarrow> config \<Rightarrow> config \<Rightarrow> bool" ("(_/ \<turnstile> (_ \<rightarrow>*/ _))" 50)
+where
+  "exec P \<equiv> star (exec1 P)"
+
+lemmas exec_induct = star.induct [of "exec1 P", split_format(complete)]
+
+code_pred exec1 by (metis exec1_def)
+
+values
+  "{(i, map t [''x'',''y''], stk) | i t stk.
+    [LOAD ''y'', STORE ''x''] \<turnstile>
+    (0, <''x'' := 3, ''y'' := 4>, []) \<rightarrow>* (i, t, stk)}"
 
 end
